now using the code from PDDL_STRIPS_Checker in Running_Example.thy

Tests.thy
@@ -1,15 +1,122 @@
 theory Tests
   imports Main
-    (* "../LTS-formalization/Datalog/Datalog"
+    "../LTS-formalization/Datalog/Datalog"
     "AI_Planning_Languages_Semantics.PDDL_STRIPS_Semantics"
     "Verified_SAT_Based_AI_Planning.STRIPS_Representation"
     "AI_Planning_Languages_Semantics.PDDL_STRIPS_Semantics"
     "HOL-Library.Monad_Syntax"
-    "HOL-Library.Multiset"*)
+    "HOL-Library.Multiset"
     
     "AI_Planning_Languages_Semantics.PDDL_STRIPS_Checker"
 begin
 
+(* define single entailment \<TTurnstile>\<^sub>1 :: formula \<Rightarrow> formula \<Rightarrow> bool *)
 
+lemma "A \<TTurnstile> B"
+
+
+
+definition "my_types \<equiv> [
+  (''City'', ''object''), (''Movable'', ''object''),
+  (''Vehicle'', ''Movable''), (''Parcel'', ''Movable''),
+  (''Car'', ''Vehicle''), (''Train'', ''Vehicle''),
+  (''R'', ''L''), (''L'', ''R''),
+  (''Batmobile'', ''Car''), (''Batmobile'', ''Train'')]"
+definition "my_type_names \<equiv> ''object'' # map fst my_types"
+(* purposely doing Car/Train instead of only Vehicle, for no reason other than to just use it somewhere *)
+definition "my_preds \<equiv> [
+  PredDecl (Pred ''at'') [Either [''Movable''], Either [''City'']],
+  PredDecl (Pred ''in'') [Either [''Parcel''], Either [''Car'', ''Train'']],
+  PredDecl (Pred ''road'') [Either [''City''], Either [''City'']],
+  PredDecl (Pred ''rails'') [Either [''City''], Either [''City'']]
+]"
+definition "my_consts \<equiv> [
+  (Obj ''A'', Either [''City'']), (Obj ''B'', Either [''City'']),
+  (Obj ''C'', Either [''City'']), (Obj ''D'', Either [''City'']),
+  (Obj ''E'', Either [''City'']), (Obj ''F'', Either [''City'']),
+  (Obj ''G'', Either [''City''])
+]"
+
+definition "op_drive \<equiv> Action_Schema ''drive''
+  [(Var ''c'', Either [''Car'']), (Var ''from'', Either [''City'']), (Var ''to'', Either [''City''])]
+  (And (Atom (predAtm (Pred ''at'') [term.VAR (Var ''c''), term.VAR (Var ''from'')]))
+     (Or (Atom (predAtm (Pred ''road'') [term.VAR (Var ''from''), term.VAR (Var ''to'')]))
+         (Atom (predAtm (Pred ''road'') [term.VAR (Var ''to''), term.VAR (Var ''from'')]))))
+  (Effect
+    [Atom (predAtm (Pred ''at'') [term.VAR (Var ''c''), term.VAR (Var ''to'')])]
+    [Atom (predAtm (Pred ''at'') [term.VAR (Var ''c''), term.VAR (Var ''from'')])])"
+definition "op_choochoo \<equiv> Action_Schema ''choochoo''
+  [(Var ''t'', Either [''Train'']), (Var ''from'', Either [''City'']), (Var ''to'', Either [''City''])]
+  (And (Atom (predAtm (Pred ''at'') [term.VAR (Var ''t''), term.VAR (Var ''from'')]))
+     (Or (Atom (predAtm (Pred ''rails'') [term.VAR (Var ''from''), term.VAR (Var ''to'')]))
+         (Atom (predAtm (Pred ''rails'') [term.VAR (Var ''to''), term.VAR (Var ''from'')]))))
+  (Effect
+    [Atom (predAtm (Pred ''at'') [term.VAR (Var ''t''), term.VAR (Var ''to'')])]
+    [Atom (predAtm (Pred ''at'') [term.VAR (Var ''t''), term.VAR (Var ''from'')])])"
+(* into has to be Car/Train instead of Vehicle because of the definition of the predicate "in" *)
+definition "op_load \<equiv> Action_Schema ''load''
+  [(Var ''what'', Either [''Parcel'']), (Var ''where'', Either [''City'']), (Var ''into'', Either [''Car'', ''Train''])]
+     (And (Atom (predAtm (Pred ''at'') [term.VAR (Var ''into''), term.VAR (Var ''where'')]))
+         (Atom (predAtm (Pred ''at'') [term.VAR (Var ''what''), term.VAR (Var ''where'')])))
+  (Effect
+    [Atom (predAtm (Pred ''in'') [term.VAR (Var ''what''), term.VAR (Var ''into'')])]
+    [Atom (predAtm (Pred ''at'') [term.VAR (Var ''what''), term.VAR (Var ''where'')])])"
+definition "op_unload \<equiv> Action_Schema ''unload''
+  [(Var ''what'', Either [''Parcel'']), (Var ''from'', Either [''Car'', ''Train'']), (Var ''where'', Either [''City''])]
+     (And (Atom (predAtm (Pred ''at'') [term.VAR (Var ''from''), term.VAR (Var ''where'')]))
+         (Atom (predAtm (Pred ''in'') [term.VAR (Var ''what''), term.VAR (Var ''from'')])))
+  (Effect
+    [Atom (predAtm (Pred ''at'') [term.VAR (Var ''what''), term.VAR (Var ''where'')])]
+    [Atom (predAtm (Pred ''in'') [term.VAR (Var ''what''), term.VAR (Var ''from'')])])"
+definition "op_broken \<equiv> Action_Schema ''broken''
+  [(Var ''x'', Either [''n'existe pas''])]
+  \<bottom>
+  (Effect [] [])" (* considered well-formed as long as x is not used in any formulas *)
+
+
+definition "my_actions \<equiv> [op_drive, op_choochoo, op_load, op_unload]"
+
+definition "my_domain \<equiv> Domain my_types my_preds my_consts my_actions"
+value "my_domain"
+(*value "ast_domain.wf_domain my_domain"*)
+
+
+(* batmobile because why not *)
+definition "my_objs \<equiv> [
+  (Obj ''c1'', Either [''Car'']),
+  (Obj ''c2'', Either [''Car'']),
+  (Obj ''c3'', Either [''Car'']),
+  (Obj ''t'', Either [''Train'']),
+  (Obj ''p1'', Either [''Parcel'']),
+  (Obj ''p2'', Either [''Parcel'']),
+  (Obj ''batmobile'', Either [''Batmobile''])
+]"
+
+definition "my_init \<equiv> [
+  Atom (predAtm (Pred ''at'') [Obj ''c1'', Obj ''A'']),
+  Atom (predAtm (Pred ''at'') [Obj ''c2'', Obj ''B'']),
+  Atom (predAtm (Pred ''at'') [Obj ''c3'', Obj ''G'']),
+  Atom (predAtm (Pred ''at'') [Obj ''t'', Obj ''E'']),
+  Atom (predAtm (Pred ''at'') [Obj ''p1'', Obj ''C'']),
+  Atom (predAtm (Pred ''at'') [Obj ''p2'', Obj ''F'']),
+  Atom (predAtm (Pred ''at'') [Obj ''batmobile'', Obj ''D'']),
+  Atom (predAtm (Pred ''road'') [Obj ''A'', Obj ''D'']),
+  Atom (predAtm (Pred ''road'') [Obj ''B'', Obj ''D'']),
+  Atom (predAtm (Pred ''road'') [Obj ''C'', Obj ''D'']),
+  Atom (predAtm (Pred ''rails'') [Obj ''D'', Obj ''E'']),
+  Atom (predAtm (Pred ''road'') [Obj ''E'', Obj ''F'']),
+  Atom (predAtm (Pred ''road'') [Obj ''F'', Obj ''G'']),
+  Atom (predAtm (Pred ''road'') [Obj ''G'', Obj ''E''])
+]"
+definition "my_goal \<equiv>
+  And (Atom (predAtm (Pred ''at'') [Obj ''p1'', Obj ''G'']))
+      (Atom (predAtm (Pred ''at'') [Obj ''p2'', Obj ''E'']))"
+
+definition "my_problem \<equiv> Problem my_domain my_objs my_init my_goal"
+
+term "ast_domain.STG my_domain"
+term "ast_domain.wf_domain' my_domain (ast_domain.STG my_domain) (ast_domain.mp_constT my_domain)"
+
+value "ast_domain.wf_domain' my_domain (ast_domain.STG my_domain) (ast_domain.mp_constT my_domain)"
 
 end
