String_Shenanigans.thy
@@ -6,6 +6,18 @@ fun max_length :: "'a list list \<Rightarrow> nat" where
   "max_length [] = 0" | (* yeah, yeah, technically it should be -1 or None/undefined or something *)
   "max_length (xs # xss) = max (length xs) (max_length xss)"
 
+thm Max_insert
+term  finite
+thm card_eq_0_iff
+
+lemma "card xs \<noteq> 0 \<Longrightarrow> Max (insert x xs) = max x (Max xs)"
+  by (metis Max_insert card.infinite card_0_eq)
+  by (simp add: card_eq_0_iff)
+
+lemma "length xss > 0 \<Longrightarrow> max_length xss = Max (set (map length xss))"
+  apply (induction xss) apply simp
+  using Max_insert card_eq_0_iff card_0_eq tr
+
 lemma max_length_correct: "\<forall>s \<in> set ss. length s \<le> max_length ss"
   by (induction ss) auto
 
